wip

ulib/FStar.Monotonic.HyperStack.fst
@@ -1,6 +1,7 @@
 module FStar.Monotonic.HyperStack
 
 open FStar.Preorder
+
 module Map = FStar.Map
 
 include FStar.Monotonic.HyperHeap
@@ -72,11 +73,24 @@ abstract let rid_ctr_pred (h:hmap) (n:int) :Type0 = rid_ctr_pred_predicate h n
 let is_wf_with_ctr_and_tip (h:hmap) (ctr:int) (tip:rid) :Type0
   = root `is_in` h /\ tip `is_tip` h /\ map_invariant h /\ downward_closed h /\ rid_ctr_pred h ctr
 
-noeq type mem =
+noeq abstract type mem =
   | HS : rid_ctr:int
          -> h:hmap
          -> tip:rid{is_wf_with_ctr_and_tip h rid_ctr tip}
          -> mem
+
+abstract let mk_mem (rid_ctr:int) (h:hmap) (tip:rid{is_wf_with_ctr_and_tip h rid_ctr tip}) :mem =
+  HS rid_ctr h tip
+
+abstract let get_hmap (m:mem) :hmap = m.h
+abstract let get_rid_ctr (m:mem) :int = m.rid_ctr
+abstract let get_tip (m:mem) :rid = m.tip
+
+private let lemma_mem_projectors_are_in_relation (m:mem)
+  :Lemma (is_wf_with_ctr_and_tip (get_hmap m) (get_rid_ctr m) (get_tip m))
+  = ()
+
+let lemma_mk_mem_and_projectors_are_inverses (rid_ctr:int) (h:hmap) (tip:
 
 private let lemma_is_wf_ctr_and_tip_intro (h:hmap) (ctr:int) (tip:rid)
   :Lemma (requires (root `is_in` h /\ (is_stack_region tip \/ tip = root) /\  tip `is_in` h /\
@@ -86,18 +100,18 @@ private let lemma_is_wf_ctr_and_tip_intro (h:hmap) (ctr:int) (tip:rid)
   = ()
 
 private let lemma_is_wf_ctr_and_tip_elim (m:mem)
-  :Lemma (requires (is_wf_with_ctr_and_tip m.h m.rid_ctr m.tip))  
-         (ensures  (root `is_in` m.h /\ (is_stack_region m.tip \/ m.tip = root) /\  m.tip `is_in` m.h /\
-	            tip_top_predicate m.tip m.h /\ map_invariant_predicate m.h /\
-                    downward_closed_predicate m.h /\ rid_ctr_pred_predicate m.h m.rid_ctr))
-  = ()
+  :Lemma (requires True)
+         (ensures  (root `is_in` get_hmap m /\ (is_stack_region (get_tip m) \/ get_tip m = root) /\  get_tip m `is_in` get_hmap m /\
+	            tip_top_predicate (get_tip m) (get_hmap m) /\ map_invariant_predicate (get_hmap m) /\
+                    downward_closed_predicate (get_hmap m) /\ rid_ctr_pred_predicate (get_hmap m) (get_rid_ctr m)))
+  = lemma_mem_projectors_are_in_relation m
 
 (******* map_invariant related lemmas ******)
 
 let lemma_map_invariant (m:mem) (r s:rid)
-  :Lemma (requires (r `is_in` m.h /\ s `is_above` r))
-         (ensures  (s `is_in` m.h))
-         [SMTPat (r `is_in` m.h); SMTPat (s `is_above` r); SMTPat (s `is_in` m.h)]
+  :Lemma (requires (r `is_in` get_hmap m /\ s `is_above` r))
+         (ensures  (s `is_in` get_hmap m))
+         [SMTPat (r `is_in` get_hmap m); SMTPat (s `is_above` r); SMTPat (s `is_in` get_hmap m)]
   = ()
 
 (******)
@@ -106,11 +120,11 @@ let lemma_map_invariant (m:mem) (r s:rid)
 (****** downward_closed related lemmas *******)
 
 let lemma_downward_closed (m:mem) (r:rid) (s:rid{s =!= root})
-  :Lemma (requires (r `is_in` m.h /\ s `is_above` r))
+  :Lemma (requires (r `is_in` get_hmap m /\ s `is_above` r))
          (ensures  (is_eternal_color (color r) == is_eternal_color (color s) /\
 	            is_stack_region r == is_stack_region s))
-         [SMTPatOr [[SMTPat (m.h `Map.contains` r); SMTPat (s `is_above` r); SMTPat (is_eternal_color (color s))];
-                    [SMTPat (m.h `Map.contains` r); SMTPat (s `is_above` r); SMTPat (is_stack_region s)]
+         [SMTPatOr [[SMTPat (get_hmap m `Map.contains` r); SMTPat (s `is_above` r); SMTPat (is_eternal_color (color s))];
+                    [SMTPat (get_hmap m `Map.contains` r); SMTPat (s `is_above` r); SMTPat (is_stack_region s)]
                     ]]
   = ()
 
@@ -119,7 +133,7 @@ let lemma_downward_closed (m:mem) (r:rid) (s:rid{s =!= root})
 (****** tip_top related lemmas ******)
 
 let lemma_tip_top (m:mem) (r:sid)
-  :Lemma (r `is_in` m.h <==> r `is_above` m.tip)
+  :Lemma (r `is_in` get_hmap m <==> r `is_above` get_tip m)
   = ()
 
 (*
@@ -129,9 +143,9 @@ let lemma_tip_top (m:mem) (r:sid)
 //  *)
 let lemma_tip_top_smt (m:mem) (r:rid)
   :Lemma (requires (is_stack_region r))
-         (ensures  (r `is_in` m.h <==> r `is_above` m.tip))
-         [SMTPatOr [[SMTPat (is_stack_region r); SMTPat (r `is_above` m.tip)];
-                    [SMTPat (is_stack_region r); SMTPat (r `is_in` m.h)]]]
+         (ensures  (r `is_in` get_hmap m <==> r `is_above` get_tip m))
+         [SMTPatOr [[SMTPat (is_stack_region r); SMTPat (r `is_above` get_tip m)];
+                    [SMTPat (is_stack_region r); SMTPat (r `is_in` get_hmap m)]]]
   = ()
 
 (******)
@@ -142,7 +156,7 @@ let lemma_tip_top_smt (m:mem) (r:rid)
 //  * Expose the meaning of the predicate itself
 //  *)
 let lemma_rid_ctr_pred ()
-  :Lemma (forall (m:mem) (r:rid).{:pattern (m.h `Map.contains` r)} m.h `Map.contains` r ==> rid_last_component r < m.rid_ctr)
+  :Lemma (forall (m:mem) (r:rid).{:pattern (get_hmap m `Map.contains` r)} get_hmap m `Map.contains` r ==> rid_last_component r < get_rid_ctr m)
   = ()
 
 (*****)
@@ -153,33 +167,33 @@ let empty_mem (m:hmap) =
   let tip = root in
   assume (rid_last_component root == 0);
   lemma_is_wf_ctr_and_tip_intro h 1 tip;
-  HS 1 h tip
+  mk_mem 1 h tip
 
-let eternal_region_does_not_overlap_with_tip (m:mem) (r:rid{is_eternal_color (color r) /\ not (disjoint r m.tip) /\ r<>root /\ is_stack_region m.tip})
+let eternal_region_does_not_overlap_with_tip (m:mem) (r:rid{is_eternal_color (color r) /\ not (disjoint r (get_tip m)) /\ r<>root /\ is_stack_region (get_tip m)})
   : Lemma (requires True)
-          (ensures (~ (r `is_in` m.h)))
+          (ensures (~ (r `is_in` (get_hmap m))))
   = root_has_color_zero()
 
-let poppable m = m.tip <> root
+let poppable m = get_tip m <> root
 
 let remove_elt (#a:eqtype) (s:Set.set a) (x:a) = Set.intersect s (Set.complement (Set.singleton x))
 
 let popped m0 m1 =
   poppable m0
-  /\ parent m0.tip = m1.tip
-  /\ Set.equal (Map.domain m1.h) (remove_elt (Map.domain m0.h) m0.tip)
-  /\ Map.equal m1.h (Map.restrict (Map.domain m1.h) m0.h)
+  /\ parent (get_tip m0) = get_tip m1
+  /\ Set.equal (Map.domain (get_hmap m1)) (remove_elt (Map.domain (get_hmap m0)) (get_tip m0))
+  /\ Map.equal (get_hmap m1) (Map.restrict (Map.domain (get_hmap m1)) (get_hmap m0))
 
 let pop (m0:mem{poppable m0}) : Tot mem =
   root_has_color_zero();
   lemma_is_wf_ctr_and_tip_elim m0;
-  let dom = remove_elt (Map.domain m0.h) m0.tip in
-  let h0 = m0.h in
-  let h1 = Map.restrict dom m0.h in
-  let tip0 = m0.tip in
+  let dom = remove_elt (Map.domain (get_hmap m0)) (get_tip m0) in
+  let h0 = get_hmap m0 in
+  let h1 = Map.restrict dom h0 in
+  let tip0 = get_tip m0 in
   let tip1 = parent tip0 in
-  lemma_is_wf_ctr_and_tip_intro h1 m0.rid_ctr tip1;
-  HS m0.rid_ctr h1 tip1
+  lemma_is_wf_ctr_and_tip_intro h1 (get_rid_ctr m0) tip1;
+  mk_mem (get_rid_ctr m0) h1 tip1
 
 //A (reference a) may reside in the stack or heap, and may be manually managed
 //Mark it private so that clients can't use its projectors etc.
@@ -244,38 +258,38 @@ let mmmref (a:Type) (rel:preorder a) =
 let s_mref (i:rid) (a:Type) (rel:preorder a) = s:mreference a rel{frameOf s = i}
 
 (*
-//  * AR: this used to be (is_eternal_region i \/ i `is_above` m.tip) /\ Map.contains ...
-//  *     As far as the memory model is concerned, this should just be Map.contains
-//  *     The fact that an eternal region is always contained (because of monotonicity) should be used in the ST interface
-//  *)
-let live_region (m:mem) (i:rid) :Tot bool = Map.contains m.h i
+// //  * AR: this used to be (is_eternal_region i \/ i `is_above` m.tip) /\ Map.contains ...
+// //  *     As far as the memory model is concerned, this should just be Map.contains
+// //  *     The fact that an eternal region is always contained (because of monotonicity) should be used in the ST interface
+// //  *)
+let live_region (m:mem) (i:rid) :Tot bool = Map.contains (get_hmap m) i
 
 let contains (#a:Type) (#rel:preorder a) (m:mem) (s:mreference a rel) :GTot bool =
   let i = frameOf s in
-  live_region m i && (FStar.StrongExcludedMiddle.strong_excluded_middle (Heap.contains (Map.sel m.h i) (as_ref s)))
+  live_region m i && (FStar.StrongExcludedMiddle.strong_excluded_middle (Heap.contains (Map.sel (get_hmap m) i) (as_ref s)))
 
 let unused_in (#a:Type) (#rel:preorder a) (r:mreference a rel) (h:mem) :GTot bool =
   let i = frameOf r in
-  not (Map.contains h.h i) ||
-  FStar.StrongExcludedMiddle.strong_excluded_middle (Heap.unused_in (as_ref r) (Map.sel h.h i))
+  not (Map.contains (get_hmap h) i) ||
+  FStar.StrongExcludedMiddle.strong_excluded_middle (Heap.unused_in (as_ref r) (Map.sel (get_hmap h) i))
 
 let contains_ref_in_its_region (#a:Type) (#rel:preorder a) (h:mem) (r:mreference a rel) :GTot bool =
   let i = frameOf r in
-  FStar.StrongExcludedMiddle.strong_excluded_middle (Heap.contains (Map.sel h.h i) (as_ref r))
+  FStar.StrongExcludedMiddle.strong_excluded_middle (Heap.contains (Map.sel (get_hmap h) i) (as_ref r))
 
 let fresh_ref (#a:Type) (#rel:preorder a) (r:mreference a rel) (m0:mem) (m1:mem) :Type0 =
   let i = frameOf r in
-  Heap.fresh (as_ref r) (Map.sel m0.h i) (Map.sel m1.h i)
+  Heap.fresh (as_ref r) (Map.sel (get_hmap m0) i) (Map.sel (get_hmap m1) i)
 
 let fresh_region (i:rid) (m0 m1:mem) =
-  not (m0.h `Map.contains` i) /\ m1.h `Map.contains` i
+  not (get_hmap m0 `Map.contains` i) /\ get_hmap m1 `Map.contains` i
 
 private val lemma_extends_fresh_disjoint: i:rid -> j:rid -> ipar:rid -> jpar:rid
-                               -> m0:mem{map_invariant m0.h} -> m1:mem{map_invariant m1.h} ->
+                               -> m0:mem{map_invariant (get_hmap m0)} -> m1:mem{map_invariant (get_hmap m1)} ->
   Lemma (requires (fresh_region i m0 m1
                   /\ fresh_region j m0 m1
-                  /\ Map.contains m0.h ipar
-                  /\ Map.contains m0.h jpar
+                  /\ Map.contains (get_hmap m0) ipar
+                  /\ Map.contains (get_hmap m0) jpar
                   /\ extends i ipar
                   /\ extends j jpar
                   /\ i<>j))
@@ -283,485 +297,485 @@ private val lemma_extends_fresh_disjoint: i:rid -> j:rid -> ipar:rid -> jpar:rid
 let lemma_extends_fresh_disjoint i j ipar jpar m0 m1 = ()
 
 (*
-//  * memory model API
-//  *)
+// //  * memory model API
+// //  *)
 let sel (#a:Type) (#rel:preorder a) (m:mem) (s:mreference a rel)
   : GTot a
-  = Heap.sel (Map.sel m.h (frameOf s)) (as_ref s)
+  = Heap.sel (Map.sel (get_hmap m) (frameOf s)) (as_ref s)
 
 let upd (#a:Type) (#rel:preorder a) (m:mem) (s:mreference a rel{live_region m (frameOf s)}) (v:a)
   : GTot mem
   = lemma_is_wf_ctr_and_tip_elim m;
     let i = frameOf s in
-    let h = Map.upd m.h i (Heap.upd (Map.sel m.h i) (as_ref s) v) in
-    lemma_is_wf_ctr_and_tip_intro h m.rid_ctr m.tip;
-    HS m.rid_ctr h m.tip
+    let h = Map.upd (get_hmap m) i (Heap.upd (Map.sel (get_hmap m) i) (as_ref s) v) in
+    lemma_is_wf_ctr_and_tip_intro h (get_rid_ctr m) (get_tip m);
+    mk_mem (get_rid_ctr m) h (get_tip m)
 
-let alloc (#a:Type0) (rel:preorder a) (id:rid) (init:a) (mm:bool) (m:mem{m.h `Map.contains` id})
-  :Tot (p:(mreference a rel * mem){let (r, h) = Heap.alloc rel (Map.sel m.h id) init mm in
+let alloc (#a:Type0) (rel:preorder a) (id:rid) (init:a) (mm:bool) (m:mem{(get_hmap m) `Map.contains` id})
+  :Tot (p:(mreference a rel * mem){let (r, h) = Heap.alloc rel (Map.sel (get_hmap m) id) init mm in
                                    as_ref (fst p) == r /\
-                                   (snd p).h == Map.upd m.h id h})
+                                   get_hmap (snd p) == Map.upd (get_hmap m) id h})
   = lemma_is_wf_ctr_and_tip_elim m;
-    let r, h = Heap.alloc rel (Map.sel m.h id) init mm in
-    let h = Map.upd m.h id h in
-    lemma_is_wf_ctr_and_tip_intro h m.rid_ctr m.tip;
-    (mk_mreference id r), (HS m.rid_ctr h m.tip)
+    let r, h = Heap.alloc rel (Map.sel (get_hmap m) id) init mm in
+    let h = Map.upd (get_hmap m) id h in
+    lemma_is_wf_ctr_and_tip_intro h (get_rid_ctr m) (get_tip m);
+    (mk_mreference id r), (mk_mem (get_rid_ctr m) h (get_tip m))
 
 let free (#a:Type0) (#rel:preorder a) (r:mreference a rel{is_mm r}) (m:mem{m `contains` r})
   :Tot mem
   = lemma_is_wf_ctr_and_tip_elim m;
     let i = frameOf r in
-    let h = Map.sel m.h i in
+    let h = Map.sel (get_hmap m) i in
     let new_h = Heap.free_mm h (as_ref r) in
-    let new_h = Map.upd m.h i new_h in
-    lemma_is_wf_ctr_and_tip_intro new_h m.rid_ctr m.tip;
-    HS m.rid_ctr new_h m.tip
-
-let upd_tot (#a:Type) (#rel:preorder a) (m:mem) (r:mreference a rel{m `contains` r}) (v:a)
-  :Tot mem
-  = lemma_is_wf_ctr_and_tip_elim m;
-    let i = frameOf r in
-    let h = Map.sel m.h i in
-    let new_h = Heap.upd_tot h (as_ref r) v in
-    let new_h = Map.upd m.h i new_h in
-    lemma_is_wf_ctr_and_tip_intro new_h m.rid_ctr m.tip;
-    HS m.rid_ctr new_h m.tip
-
-let sel_tot (#a:Type) (#rel:preorder a) (m:mem) (r:mreference a rel{m `contains` r})
-  :Tot a
-  = Heap.sel_tot (Map.sel m.h (frameOf r)) (as_ref r)
-
-let fresh_frame (m0:mem) (m1:mem) =
-  not (Map.contains m0.h m1.tip) /\
-  parent m1.tip = m0.tip         /\
-  m1.h == Map.upd m0.h m1.tip Heap.emp
-
-let hs_push_frame (m:mem) :Tot (m':mem{fresh_frame m m'})
-  = lemma_is_wf_ctr_and_tip_elim m;
-    let new_tip_rid = extend m.tip m.rid_ctr 1 in
-    let h = Map.upd m.h new_tip_rid Heap.emp in
-    assert (forall (s:rid). (new_tip_rid `is_above` s /\ s `is_in` h) ==> s = new_tip_rid);
-    lemma_is_wf_ctr_and_tip_intro h (m.rid_ctr + 1) new_tip_rid;
-    HS (m.rid_ctr + 1) h new_tip_rid
-
-let new_eternal_region (m:mem) (parent:rid{is_eternal_color (color parent) /\ m.h `Map.contains` parent})
-                       (c:option int{None? c \/ is_eternal_color (Some?.v c)})
-  :Tot (t:(rid * mem){fresh_region (fst t) m (snd t)})
-  = lemma_is_wf_ctr_and_tip_elim m;
-    let new_rid =
-      if None? c then extend_monochrome parent m.rid_ctr
-      else extend parent m.rid_ctr (Some?.v c)
-    in
-    let h1 = Map.upd m.h new_rid Heap.emp in
-    lemma_is_wf_ctr_and_tip_intro h1 (m.rid_ctr + 1) m.tip;
-    new_rid, HS (m.rid_ctr + 1) h1 m.tip
-
-(****** The following two lemmas are only used in FStar.Pointer.Base, and invoked explicitly ******)
-
-let lemma_sel_same_addr (#a:Type0) (#rel:preorder a) (h:mem) (r1:mreference a rel) (r2:mreference a rel)
-  :Lemma (requires (frameOf r1 == frameOf r2 /\ h `contains` r1 /\ as_addr r1 = as_addr r2 /\ is_mm r1 == is_mm r2))
-         (ensures  (h `contains` r2 /\ sel h r1 == sel h r2))
-  = Heap.lemma_sel_same_addr (Map.sel h.h (frameOf r1)) (as_ref r1) (as_ref r2)
-
-let lemma_upd_same_addr (#a:Type0) (#rel:preorder a) (h:mem) (r1 r2:mreference a rel) (x: a)
-  :Lemma (requires (frameOf r1 == frameOf r2 /\ (h `contains` r1 \/ h `contains` r2) /\
-                    as_addr r1 == as_addr r2 /\ is_mm r1 == is_mm r2))
-         (ensures  (h `contains` r1 /\ h `contains` r2 /\ upd h r1 x == upd h r2 x))
-  = FStar.Monotonic.Heap.lemma_heap_equality_upd_same_addr (Map.sel h.h (frameOf r1)) (as_ref r1) (as_ref r2) x;
-    if StrongExcludedMiddle.strong_excluded_middle (h `contains` r1) then
-      lemma_sel_same_addr h r1 r2
-    else lemma_sel_same_addr h r2 r1
-
-(* Two references with different reads are disjoint. *)
-
-let mreference_distinct_sel_disjoint
-  (#a:Type0) (#rel1: preorder a) (#rel2: preorder a) (h: mem) (r1: mreference a rel1) (r2:mreference a rel2)
-: Lemma
-  (requires (
-    h `contains` r1 /\
-    h `contains` r2 /\
-    frameOf r1 == frameOf r2 /\
-    as_addr r1 == as_addr r2
-  ))
-  (ensures (
-    sel h r1 == sel h r2
-  ))
-= Heap.lemma_distinct_addrs_distinct_preorders ();
-  Heap.lemma_distinct_addrs_distinct_mm ();
-  Heap.lemma_sel_same_addr #a #rel1 (Map.sel h.h (frameOf r1)) (as_ref r1) (as_ref r2)
-
-(*
-// //  * AR: 12/26: modifies clauses
-// //  *            NOTE: the modifies clauses used to have a m0.tip == m1.tip conjunct too
-// //  *                  which seemed a bit misplaced
-// //  *                  removing that conjunct required very few changes (one in HACL), since ST effect gives it already
-// //  *)
-let modifies (s:Set.set rid) (m0:mem) (m1:mem) =
-  modifies_just s m0.h m1.h
-
-let modifies_transitively (s:Set.set rid) (m0:mem) (m1:mem) =
-  FStar.Monotonic.HyperHeap.modifies s m0.h m1.h
-
-let heap_only (m0:mem) = m0.tip = root
-
-let top_frame (m:mem) = Map.sel m.h m.tip
-
-let modifies_drop_tip (m0:mem) (m1:mem) (m2:mem) (s:Set.set rid)
-    : Lemma (fresh_frame m0 m1 /\ m1.tip == m2.tip /\
-             modifies_transitively (Set.union s (Set.singleton m1.tip)) m1 m2 ==>
-             modifies_transitively s m0 (pop m2))
-    = ()
-
-private let lemma_pop_is_popped (m0:mem{poppable m0})
-  : Lemma (popped m0 (pop m0))
-  = let m1 = pop m0 in
-    assert (Set.equal (Map.domain m1.h) (remove_elt (Map.domain m0.h) m0.tip))
-
-let modifies_one id h0 h1 = modifies_one id h0.h h1.h
-let modifies_ref (id:rid) (s:Set.set nat) (h0:mem) (h1:mem) =
-  Heap.modifies s (Map.sel h0.h id) (Map.sel h1.h id)
-
-private let lemma_upd_1 #a #rel (h:mem) (x:mreference a rel) (v:a{rel (sel h x) v}) : Lemma
-  (requires (contains h x))
-  (ensures (contains h x
-            /\ modifies_one (frameOf x) h (upd h x v)
-            /\ modifies_ref (frameOf x) (Set.singleton (as_addr x)) h (upd h x v)
-            /\ sel (upd h x v) x == v ))
-  = ()
-
-private let lemma_upd_2 (#a:Type) (#rel:preorder a) (h:mem) (x:mreference a rel) (v:a{rel (sel h x) v}) : Lemma
-  (requires (frameOf x = h.tip /\ x `unused_in` h))
-  (ensures (frameOf x = h.tip
-            /\ modifies_one h.tip h (upd h x v)
-            /\ modifies_ref h.tip Set.empty h (upd h x v)
-            /\ sel (upd h x v) x == v ))
-  = ()
-
-private val lemma_live_1: #a:Type ->  #a':Type -> #rel:preorder a -> #rel':preorder a'
-                  -> h:mem -> x:mreference a rel -> x':mreference a' rel' -> Lemma
-  (requires (contains h x /\ x' `unused_in` h))
-  (ensures  (frameOf x <> frameOf x' \/ ~ (as_ref x === as_ref x')))
-let lemma_live_1 #a #a' #rel #rel' h x x' = ()
-
-let above_tip_is_live (#a:Type) (#rel:preorder a) (m:mem) (x:mreference a rel) : Lemma
-  (requires (frameOf x `is_above` m.tip))
-  (ensures (frameOf x `is_in` m.h))
-  = ()
-
-noeq type some_ref =
-  | Ref : #a:Type0 -> #rel:preorder a -> mreference a rel -> some_ref
-
-let some_refs = list some_ref
-
-[@"opaque_to_smt"]
-private let rec regions_of_some_refs (rs:some_refs) :Tot (Set.set rid) =
-  match rs with
-  | []         -> Set.empty
-  | (Ref r)::tl -> Set.union (Set.singleton (frameOf r)) (regions_of_some_refs tl)
-
-[@"opaque_to_smt"]
-private let rec refs_in_region (r:rid) (rs:some_refs) :GTot (Set.set nat) =
-  match rs with
-  | []         -> Set.empty
-  | (Ref x)::tl ->
-    Set.union (if frameOf x = r then Set.singleton (as_addr x) else Set.empty)
-              (refs_in_region r tl)
-
-[@"opaque_to_smt"]
-private let rec modifies_some_refs (i:some_refs) (rs:some_refs) (h0:mem) (h1:mem) :GTot Type0 =
-  match i with
-  | []         -> True
-  | (Ref x)::tl ->
-    (modifies_ref (frameOf x) (refs_in_region (frameOf x) rs) h0 h1) /\
-    (modifies_some_refs tl rs h0 h1)
-
-[@"opaque_to_smt"]
-unfold private let norm_steps :list norm_step =
-  //iota for reducing match
-  [iota; zeta; delta; delta_only ["FStar.Monotonic.HyperStack.regions_of_some_refs";
-                            "FStar.Monotonic.HyperStack.refs_in_region";
-                            "FStar.Monotonic.HyperStack.modifies_some_refs"];
-   primops]
-
-[@"opaque_to_smt"]
-unfold let mods (rs:some_refs) (h0 h1:mem) :GTot Type0 =
-  (norm norm_steps (modifies (regions_of_some_refs rs) h0 h1)) /\
-  (norm norm_steps (modifies_some_refs rs rs h0 h1))
-
-////////////////////////////////////////////////////////////////////////////////
-let eternal_disjoint_from_tip (h:mem{is_stack_region h.tip})
-                              (r:rid{is_eternal_color (color r) /\
-                                     r<>root /\
-                                     r `is_in` h.h})
-   : Lemma (disjoint h.tip r)
-   = ()
-
-////////////////////////////////////////////////////////////////////////////////
-
-let lemma_heap_equality_cancel_same_mref_upd
-  (#a:Type) (#rel:preorder a) (h:mem) (r:mreference a rel) (x y:a)
-  :Lemma (requires (live_region h (frameOf r)))
-         (ensures  (upd (upd h r x) r y == upd h r y))
-  = let h0 = upd (upd h r x) r y in
-    let h1 = upd h r y in
-    Heap.lemma_heap_equality_cancel_same_mref_upd (Map.sel h.h (frameOf r)) (as_ref r) x y;
-    assert (Map.equal h0.h h1.h)
-
-let lemma_heap_equality_upd_with_sel
-  (#a:Type) (#rel:preorder a) (h:mem) (r:mreference a rel)
-  :Lemma (requires (h `contains` r))
-         (ensures  (upd h r (sel h r) == h))
-  = let h' = upd h r (sel h r) in
-    Heap.lemma_heap_equality_upd_with_sel (Map.sel h.h (frameOf r)) (as_ref r);
-    assert (Map.equal h.h h'.h)
-
-let lemma_heap_equality_commute_distinct_upds
-  (#a:Type) (#b:Type) (#rel_a:preorder a) (#rel_b:preorder b)
-  (h:mem) (r1:mreference a rel_a) (r2:mreference b rel_b) (x:a) (y:b)
-  :Lemma (requires (as_addr r1 =!= as_addr r2 /\ live_region h (frameOf r1) /\ live_region h (frameOf r2)))
-         (ensures  (upd (upd h r1 x) r2 y == upd (upd h r2 y) r1 x))
-  = let h0 = upd (upd h r1 x) r2 y in
-    let h1 = upd (upd h r2 y) r1 x in
-    if frameOf r1 = frameOf r2 then Heap.lemma_heap_equality_commute_distinct_upds (Map.sel h.h (frameOf r1)) (as_ref r1) (as_ref r2) x y;
-    assert (Map.equal h0.h h1.h)
-
-(*** Untyped views of references *)
-
-(* Definition and ghost decidable equality *)
-
-noeq abstract type aref: Type0 =
-| ARef:
-    (aref_region: rid) ->
-    (aref_aref: Heap.aref) ->
-    aref
-
-abstract let dummy_aref : aref = ARef root Heap.dummy_aref
-
-abstract let aref_equal
-  (a1 a2: aref)
-: Ghost bool
-  (requires True)
-  (ensures (fun b -> b == true <==> a1 == a2))
-= a1.aref_region = a2.aref_region && Heap.aref_equal a1.aref_aref a2.aref_aref
-
-(* Introduction rule *)
-
-abstract let aref_of
-  (#t: Type)
-  (#rel: preorder t)
-  (r: mreference t rel)
-  : Tot aref
-  = ARef (frameOf r) (Heap.aref_of (as_ref r))
-
-(* Operators lifted from reference *)
-
-abstract let frameOf_aref
-  (a: aref)
-: GTot rid
-= a.aref_region
-
-abstract let frameOf_aref_of
-  (#t: Type)
-  (#rel: preorder t)
-  (r: mreference t rel)
-: Lemma
-  (frameOf_aref (aref_of r) == frameOf r)
-  [SMTPat (frameOf_aref (aref_of r))]
-= ()
-
-abstract let aref_as_addr
-  (a: aref)
-: GTot (x: nat { x > 0 } )
-= Heap.addr_of_aref a.aref_aref
-
-abstract let aref_as_addr_aref_of
-  (#t: Type)
-  (#rel: preorder t)
-  (r: mreference t rel)
-: Lemma
-  (aref_as_addr (aref_of r) == as_addr r)
-  [SMTPat (aref_as_addr (aref_of r))]
-= Heap.addr_of_aref_of (as_ref r)
-
-abstract let aref_is_mm
-  (r: aref)
-: GTot bool
-= Heap.aref_is_mm r.aref_aref
-
-abstract let is_mm_aref_of
-  (#t: Type)
-  (#rel: preorder t)
-  (r: mreference t rel)
-: Lemma
-  (aref_is_mm (aref_of r) == is_mm r)
-  [SMTPat (aref_is_mm (aref_of r))]
-= Heap.is_mm_aref_of (as_ref r)
-
-abstract let aref_unused_in
-  (a: aref)
-  (h: mem)
-: GTot Type0
-= ~ (live_region h a.aref_region) \/
-  Heap.aref_unused_in a.aref_aref (Map.sel h.h a.aref_region)
-
-abstract let unused_in_aref_of
-  (#t: Type)
-  (#rel: preorder t)
-  (r: mreference t rel)
-  (h: mem)
-: Lemma
-  (aref_unused_in (aref_of r) h <==> unused_in r h)
-  [SMTPat (aref_unused_in (aref_of r) h)]
-= Heap.unused_in_aref_of (as_ref r) (Map.sel h.h (frameOf r))
-
-abstract
-val contains_aref_unused_in: #a:Type -> #rel: preorder a -> h:mem -> x:mreference a rel -> y:aref -> Lemma
-  (requires (contains h x /\ aref_unused_in y h))
-  (ensures  (frameOf x <> frameOf_aref y \/ as_addr x <> aref_as_addr y))
-  [SMTPat (contains h x); SMTPat (aref_unused_in y h)]
-let contains_aref_unused_in #a #rel h x y =
-  if frameOf x = frameOf_aref y
-  then
-    Heap.contains_aref_unused_in (Map.sel h.h (frameOf x)) (as_ref x) y.aref_aref
-  else ()
-
-(* Elimination rule *)
-
-abstract
-let aref_live_at
-  (h: mem)
-  (a: aref)
-  (v: Type)
-  (rel: preorder v)
-: GTot Type0
-= live_region h a.aref_region
-  /\ Heap.aref_live_at (Map.sel h.h a.aref_region) a.aref_aref v rel
-
-abstract
-let greference_of
-  (a: aref)
-  (v: Type)
-  (rel: preorder v)
-: Ghost (mreference v rel)
-  (requires (exists h . aref_live_at h a v rel))
-  (ensures (fun _ -> True))
-= MkRef a.aref_region (Heap.gref_of a.aref_aref v rel)
-
-abstract
-let reference_of
-  (h: mem)
-  (a: aref)
-  (v: Type)
-  (rel: preorder v)
-: Pure (mreference v rel)
-  (requires (aref_live_at h a v rel))
-  (ensures (fun x -> aref_live_at h a v rel /\ frameOf x == frameOf_aref a /\ as_addr x == aref_as_addr a /\ is_mm x == aref_is_mm a))
-= MkRef a.aref_region (Heap.ref_of (Map.sel h.h a.aref_region) a.aref_aref v rel)
-
-abstract
-let aref_live_at_aref_of
-  (h: mem)
-  (#t: Type0)
-  (#rel: preorder t)
-  (r: mreference t rel)
-: Lemma
-  (aref_live_at h (aref_of r) t rel <==> contains h r)
-  [SMTPat (aref_live_at h (aref_of r) t rel)]
-= ()
-
-abstract
-let contains_greference_of
-  (h: mem)
-  (a: aref)
-  (t: Type0)
-  (rel: preorder t)
-: Lemma
-  (requires (exists h' . aref_live_at h' a t rel))
-  (ensures ((exists h' . aref_live_at h' a t rel) /\ (contains h (greference_of a t rel) <==> aref_live_at h a t rel)))
-  [SMTPatOr [
-    [SMTPat (contains h (greference_of a t rel))];
-    [SMTPat (aref_live_at h a t rel)];
-  ]]
-= ()
-
-abstract
-let aref_of_greference_of
-  (a: aref)
-  (v: Type0)
-  (rel: preorder v)
-: Lemma
-  (requires (exists h' . aref_live_at h' a v rel))
-  (ensures ((exists h' . aref_live_at h' a v rel) /\ aref_of (greference_of a v rel) == a))
-  [SMTPat (aref_of (greference_of a v rel))]
-= ()
-
-(* Operators lowered to rref *)
-
-abstract let frameOf_greference_of
-  (a: aref)
-  (t: Type)
-  (rel: preorder t)
-: Lemma
-  (requires (exists h . aref_live_at h a t rel))
-  (ensures ((exists h . aref_live_at h a t rel) /\ frameOf (greference_of a t rel) == frameOf_aref a))
-  [SMTPat (frameOf (greference_of a t rel))]
-= ()
-
-abstract
-let as_addr_greference_of
-  (a: aref)
-  (t: Type0)
-  (rel: preorder t)
-: Lemma
-  (requires (exists h . aref_live_at h a t rel))
-  (ensures ((exists h . aref_live_at h a t rel) /\ as_addr (greference_of a t rel) == aref_as_addr a))
-  [SMTPat (as_addr (greference_of a t rel))]
-= ()
-
-abstract
-let is_mm_greference_of
-  (a: aref)
-  (t: Type0)
-  (rel: preorder t)
-: Lemma
-  (requires (exists h . aref_live_at h a t rel))
-  (ensures ((exists h . aref_live_at h a t rel) /\ is_mm (greference_of a t rel) == aref_is_mm a))
-  [SMTPat (is_mm (greference_of a t rel))]
-= ()
-
-abstract
-let unused_in_greference_of
-  (a: aref)
-  (t: Type0)
-  (rel: preorder t)
-  (h: mem)
-: Lemma
-  (requires (exists h . aref_live_at h a t rel))
-  (ensures ((exists h . aref_live_at h a t rel) /\ (unused_in (greference_of a t rel) h <==> aref_unused_in a h)))
-  [SMTPat (unused_in (greference_of a t rel) h)]
-= ()
-
-abstract
-let sel_reference_of
-  (a: aref)
-  (v: Type0)
-  (rel: preorder v)
-  (h1 h2: mem)
-: Lemma
-  (requires (aref_live_at h1 a v rel /\ aref_live_at h2 a v rel))
-  (ensures (aref_live_at h2 a v rel /\ sel h1 (reference_of h2 a v rel) == sel h1 (greference_of a v rel)))
-  [SMTPat (sel h1 (reference_of h2 a v rel))]
-= ()
-
-abstract
-let upd_reference_of
-  (a: aref)
-  (v: Type0)
-  (rel: preorder v)
-  (h1 h2: mem)
-  (x: v)
-: Lemma
-  (requires (aref_live_at h1 a v rel /\ aref_live_at h2 a v rel))
-  (ensures (aref_live_at h1 a v rel /\ aref_live_at h2 a v rel /\ upd h1 (reference_of h2 a v rel) x == upd h1 (greference_of a v rel) x))
-  [SMTPat (upd h1 (reference_of h2 a v rel) x)]
-= ()
+    let new_h = Map.upd (get_hmap m) i new_h in
+    lemma_is_wf_ctr_and_tip_intro new_h (get_rid_ctr m) (get_tip m);
+    mk_mem (get_rid_ctr m) new_h (get_tip m)
+
+// let upd_tot (#a:Type) (#rel:preorder a) (m:mem) (r:mreference a rel{m `contains` r}) (v:a)
+//   :Tot mem
+//   = lemma_is_wf_ctr_and_tip_elim m;
+//     let i = frameOf r in
+//     let h = Map.sel m.h i in
+//     let new_h = Heap.upd_tot h (as_ref r) v in
+//     let new_h = Map.upd m.h i new_h in
+//     lemma_is_wf_ctr_and_tip_intro new_h m.rid_ctr m.tip;
+//     HS m.rid_ctr new_h m.tip
+
+// let sel_tot (#a:Type) (#rel:preorder a) (m:mem) (r:mreference a rel{m `contains` r})
+//   :Tot a
+//   = Heap.sel_tot (Map.sel m.h (frameOf r)) (as_ref r)
+
+// let fresh_frame (m0:mem) (m1:mem) =
+//   not (Map.contains m0.h m1.tip) /\
+//   parent m1.tip = m0.tip         /\
+//   m1.h == Map.upd m0.h m1.tip Heap.emp
+
+// let hs_push_frame (m:mem) :Tot (m':mem{fresh_frame m m'})
+//   = lemma_is_wf_ctr_and_tip_elim m;
+//     let new_tip_rid = extend m.tip m.rid_ctr 1 in
+//     let h = Map.upd m.h new_tip_rid Heap.emp in
+//     assert (forall (s:rid). (new_tip_rid `is_above` s /\ s `is_in` h) ==> s = new_tip_rid);
+//     lemma_is_wf_ctr_and_tip_intro h (m.rid_ctr + 1) new_tip_rid;
+//     HS (m.rid_ctr + 1) h new_tip_rid
+
+// let new_eternal_region (m:mem) (parent:rid{is_eternal_color (color parent) /\ m.h `Map.contains` parent})
+//                        (c:option int{None? c \/ is_eternal_color (Some?.v c)})
+//   :Tot (t:(rid * mem){fresh_region (fst t) m (snd t)})
+//   = lemma_is_wf_ctr_and_tip_elim m;
+//     let new_rid =
+//       if None? c then extend_monochrome parent m.rid_ctr
+//       else extend parent m.rid_ctr (Some?.v c)
+//     in
+//     let h1 = Map.upd m.h new_rid Heap.emp in
+//     lemma_is_wf_ctr_and_tip_intro h1 (m.rid_ctr + 1) m.tip;
+//     new_rid, HS (m.rid_ctr + 1) h1 m.tip
+
+// (****** The following two lemmas are only used in FStar.Pointer.Base, and invoked explicitly ******)
+
+// let lemma_sel_same_addr (#a:Type0) (#rel:preorder a) (h:mem) (r1:mreference a rel) (r2:mreference a rel)
+//   :Lemma (requires (frameOf r1 == frameOf r2 /\ h `contains` r1 /\ as_addr r1 = as_addr r2 /\ is_mm r1 == is_mm r2))
+//          (ensures  (h `contains` r2 /\ sel h r1 == sel h r2))
+//   = Heap.lemma_sel_same_addr (Map.sel h.h (frameOf r1)) (as_ref r1) (as_ref r2)
+
+// let lemma_upd_same_addr (#a:Type0) (#rel:preorder a) (h:mem) (r1 r2:mreference a rel) (x: a)
+//   :Lemma (requires (frameOf r1 == frameOf r2 /\ (h `contains` r1 \/ h `contains` r2) /\
+//                     as_addr r1 == as_addr r2 /\ is_mm r1 == is_mm r2))
+//          (ensures  (h `contains` r1 /\ h `contains` r2 /\ upd h r1 x == upd h r2 x))
+//   = FStar.Monotonic.Heap.lemma_heap_equality_upd_same_addr (Map.sel h.h (frameOf r1)) (as_ref r1) (as_ref r2) x;
+//     if StrongExcludedMiddle.strong_excluded_middle (h `contains` r1) then
+//       lemma_sel_same_addr h r1 r2
+//     else lemma_sel_same_addr h r2 r1
+
+// (* Two references with different reads are disjoint. *)
+
+// let mreference_distinct_sel_disjoint
+//   (#a:Type0) (#rel1: preorder a) (#rel2: preorder a) (h: mem) (r1: mreference a rel1) (r2:mreference a rel2)
+// : Lemma
+//   (requires (
+//     h `contains` r1 /\
+//     h `contains` r2 /\
+//     frameOf r1 == frameOf r2 /\
+//     as_addr r1 == as_addr r2
+//   ))
+//   (ensures (
+//     sel h r1 == sel h r2
+//   ))
+// = Heap.lemma_distinct_addrs_distinct_preorders ();
+//   Heap.lemma_distinct_addrs_distinct_mm ();
+//   Heap.lemma_sel_same_addr #a #rel1 (Map.sel h.h (frameOf r1)) (as_ref r1) (as_ref r2)
+
+// (*
+// // //  * AR: 12/26: modifies clauses
+// // //  *            NOTE: the modifies clauses used to have a m0.tip == m1.tip conjunct too
+// // //  *                  which seemed a bit misplaced
+// // //  *                  removing that conjunct required very few changes (one in HACL), since ST effect gives it already
+// // //  *)
+// let modifies (s:Set.set rid) (m0:mem) (m1:mem) =
+//   modifies_just s m0.h m1.h
+
+// let modifies_transitively (s:Set.set rid) (m0:mem) (m1:mem) =
+//   FStar.Monotonic.HyperHeap.modifies s m0.h m1.h
+
+// let heap_only (m0:mem) = m0.tip = root
+
+// let top_frame (m:mem) = Map.sel m.h m.tip
+
+// let modifies_drop_tip (m0:mem) (m1:mem) (m2:mem) (s:Set.set rid)
+//     : Lemma (fresh_frame m0 m1 /\ m1.tip == m2.tip /\
+//              modifies_transitively (Set.union s (Set.singleton m1.tip)) m1 m2 ==>
+//              modifies_transitively s m0 (pop m2))
+//     = ()
+
+// private let lemma_pop_is_popped (m0:mem{poppable m0})
+//   : Lemma (popped m0 (pop m0))
+//   = let m1 = pop m0 in
+//     assert (Set.equal (Map.domain m1.h) (remove_elt (Map.domain m0.h) m0.tip))
+
+// let modifies_one id h0 h1 = modifies_one id h0.h h1.h
+// let modifies_ref (id:rid) (s:Set.set nat) (h0:mem) (h1:mem) =
+//   Heap.modifies s (Map.sel h0.h id) (Map.sel h1.h id)
+
+// private let lemma_upd_1 #a #rel (h:mem) (x:mreference a rel) (v:a{rel (sel h x) v}) : Lemma
+//   (requires (contains h x))
+//   (ensures (contains h x
+//             /\ modifies_one (frameOf x) h (upd h x v)
+//             /\ modifies_ref (frameOf x) (Set.singleton (as_addr x)) h (upd h x v)
+//             /\ sel (upd h x v) x == v ))
+//   = ()
+
+// private let lemma_upd_2 (#a:Type) (#rel:preorder a) (h:mem) (x:mreference a rel) (v:a{rel (sel h x) v}) : Lemma
+//   (requires (frameOf x = h.tip /\ x `unused_in` h))
+//   (ensures (frameOf x = h.tip
+//             /\ modifies_one h.tip h (upd h x v)
+//             /\ modifies_ref h.tip Set.empty h (upd h x v)
+//             /\ sel (upd h x v) x == v ))
+//   = ()
+
+// private val lemma_live_1: #a:Type ->  #a':Type -> #rel:preorder a -> #rel':preorder a'
+//                   -> h:mem -> x:mreference a rel -> x':mreference a' rel' -> Lemma
+//   (requires (contains h x /\ x' `unused_in` h))
+//   (ensures  (frameOf x <> frameOf x' \/ ~ (as_ref x === as_ref x')))
+// let lemma_live_1 #a #a' #rel #rel' h x x' = ()
+
+// let above_tip_is_live (#a:Type) (#rel:preorder a) (m:mem) (x:mreference a rel) : Lemma
+//   (requires (frameOf x `is_above` m.tip))
+//   (ensures (frameOf x `is_in` m.h))
+//   = ()
+
+// noeq type some_ref =
+//   | Ref : #a:Type0 -> #rel:preorder a -> mreference a rel -> some_ref
+
+// let some_refs = list some_ref
+
+// [@"opaque_to_smt"]
+// private let rec regions_of_some_refs (rs:some_refs) :Tot (Set.set rid) =
+//   match rs with
+//   | []         -> Set.empty
+//   | (Ref r)::tl -> Set.union (Set.singleton (frameOf r)) (regions_of_some_refs tl)
+
+// [@"opaque_to_smt"]
+// private let rec refs_in_region (r:rid) (rs:some_refs) :GTot (Set.set nat) =
+//   match rs with
+//   | []         -> Set.empty
+//   | (Ref x)::tl ->
+//     Set.union (if frameOf x = r then Set.singleton (as_addr x) else Set.empty)
+//               (refs_in_region r tl)
+
+// [@"opaque_to_smt"]
+// private let rec modifies_some_refs (i:some_refs) (rs:some_refs) (h0:mem) (h1:mem) :GTot Type0 =
+//   match i with
+//   | []         -> True
+//   | (Ref x)::tl ->
+//     (modifies_ref (frameOf x) (refs_in_region (frameOf x) rs) h0 h1) /\
+//     (modifies_some_refs tl rs h0 h1)
+
+// [@"opaque_to_smt"]
+// unfold private let norm_steps :list norm_step =
+//   //iota for reducing match
+//   [iota; zeta; delta; delta_only ["FStar.Monotonic.HyperStack.regions_of_some_refs";
+//                             "FStar.Monotonic.HyperStack.refs_in_region";
+//                             "FStar.Monotonic.HyperStack.modifies_some_refs"];
+//    primops]
+
+// [@"opaque_to_smt"]
+// unfold let mods (rs:some_refs) (h0 h1:mem) :GTot Type0 =
+//   (norm norm_steps (modifies (regions_of_some_refs rs) h0 h1)) /\
+//   (norm norm_steps (modifies_some_refs rs rs h0 h1))
+
+// ////////////////////////////////////////////////////////////////////////////////
+// let eternal_disjoint_from_tip (h:mem{is_stack_region h.tip})
+//                               (r:rid{is_eternal_color (color r) /\
+//                                      r<>root /\
+//                                      r `is_in` h.h})
+//    : Lemma (disjoint h.tip r)
+//    = ()
+
+// ////////////////////////////////////////////////////////////////////////////////
+
+// let lemma_heap_equality_cancel_same_mref_upd
+//   (#a:Type) (#rel:preorder a) (h:mem) (r:mreference a rel) (x y:a)
+//   :Lemma (requires (live_region h (frameOf r)))
+//          (ensures  (upd (upd h r x) r y == upd h r y))
+//   = let h0 = upd (upd h r x) r y in
+//     let h1 = upd h r y in
+//     Heap.lemma_heap_equality_cancel_same_mref_upd (Map.sel h.h (frameOf r)) (as_ref r) x y;
+//     assert (Map.equal h0.h h1.h)
+
+// let lemma_heap_equality_upd_with_sel
+//   (#a:Type) (#rel:preorder a) (h:mem) (r:mreference a rel)
+//   :Lemma (requires (h `contains` r))
+//          (ensures  (upd h r (sel h r) == h))
+//   = let h' = upd h r (sel h r) in
+//     Heap.lemma_heap_equality_upd_with_sel (Map.sel h.h (frameOf r)) (as_ref r);
+//     assert (Map.equal h.h h'.h)
+
+// let lemma_heap_equality_commute_distinct_upds
+//   (#a:Type) (#b:Type) (#rel_a:preorder a) (#rel_b:preorder b)
+//   (h:mem) (r1:mreference a rel_a) (r2:mreference b rel_b) (x:a) (y:b)
+//   :Lemma (requires (as_addr r1 =!= as_addr r2 /\ live_region h (frameOf r1) /\ live_region h (frameOf r2)))
+//          (ensures  (upd (upd h r1 x) r2 y == upd (upd h r2 y) r1 x))
+//   = let h0 = upd (upd h r1 x) r2 y in
+//     let h1 = upd (upd h r2 y) r1 x in
+//     if frameOf r1 = frameOf r2 then Heap.lemma_heap_equality_commute_distinct_upds (Map.sel h.h (frameOf r1)) (as_ref r1) (as_ref r2) x y;
+//     assert (Map.equal h0.h h1.h)
+
+// (*** Untyped views of references *)
+
+// (* Definition and ghost decidable equality *)
+
+// noeq abstract type aref: Type0 =
+// | ARef:
+//     (aref_region: rid) ->
+//     (aref_aref: Heap.aref) ->
+//     aref
+
+// abstract let dummy_aref : aref = ARef root Heap.dummy_aref
+
+// abstract let aref_equal
+//   (a1 a2: aref)
+// : Ghost bool
+//   (requires True)
+//   (ensures (fun b -> b == true <==> a1 == a2))
+// = a1.aref_region = a2.aref_region && Heap.aref_equal a1.aref_aref a2.aref_aref
+
+// (* Introduction rule *)
+
+// abstract let aref_of
+//   (#t: Type)
+//   (#rel: preorder t)
+//   (r: mreference t rel)
+//   : Tot aref
+//   = ARef (frameOf r) (Heap.aref_of (as_ref r))
+
+// (* Operators lifted from reference *)
+
+// abstract let frameOf_aref
+//   (a: aref)
+// : GTot rid
+// = a.aref_region
+
+// abstract let frameOf_aref_of
+//   (#t: Type)
+//   (#rel: preorder t)
+//   (r: mreference t rel)
+// : Lemma
+//   (frameOf_aref (aref_of r) == frameOf r)
+//   [SMTPat (frameOf_aref (aref_of r))]
+// = ()
+
+// abstract let aref_as_addr
+//   (a: aref)
+// : GTot (x: nat { x > 0 } )
+// = Heap.addr_of_aref a.aref_aref
+
+// abstract let aref_as_addr_aref_of
+//   (#t: Type)
+//   (#rel: preorder t)
+//   (r: mreference t rel)
+// : Lemma
+//   (aref_as_addr (aref_of r) == as_addr r)
+//   [SMTPat (aref_as_addr (aref_of r))]
+// = Heap.addr_of_aref_of (as_ref r)
+
+// abstract let aref_is_mm
+//   (r: aref)
+// : GTot bool
+// = Heap.aref_is_mm r.aref_aref
+
+// abstract let is_mm_aref_of
+//   (#t: Type)
+//   (#rel: preorder t)
+//   (r: mreference t rel)
+// : Lemma
+//   (aref_is_mm (aref_of r) == is_mm r)
+//   [SMTPat (aref_is_mm (aref_of r))]
+// = Heap.is_mm_aref_of (as_ref r)
+
+// abstract let aref_unused_in
+//   (a: aref)
+//   (h: mem)
+// : GTot Type0
+// = ~ (live_region h a.aref_region) \/
+//   Heap.aref_unused_in a.aref_aref (Map.sel h.h a.aref_region)
+
+// abstract let unused_in_aref_of
+//   (#t: Type)
+//   (#rel: preorder t)
+//   (r: mreference t rel)
+//   (h: mem)
+// : Lemma
+//   (aref_unused_in (aref_of r) h <==> unused_in r h)
+//   [SMTPat (aref_unused_in (aref_of r) h)]
+// = Heap.unused_in_aref_of (as_ref r) (Map.sel h.h (frameOf r))
+
+// abstract
+// val contains_aref_unused_in: #a:Type -> #rel: preorder a -> h:mem -> x:mreference a rel -> y:aref -> Lemma
+//   (requires (contains h x /\ aref_unused_in y h))
+//   (ensures  (frameOf x <> frameOf_aref y \/ as_addr x <> aref_as_addr y))
+//   [SMTPat (contains h x); SMTPat (aref_unused_in y h)]
+// let contains_aref_unused_in #a #rel h x y =
+//   if frameOf x = frameOf_aref y
+//   then
+//     Heap.contains_aref_unused_in (Map.sel h.h (frameOf x)) (as_ref x) y.aref_aref
+//   else ()
+
+// (* Elimination rule *)
+
+// abstract
+// let aref_live_at
+//   (h: mem)
+//   (a: aref)
+//   (v: Type)
+//   (rel: preorder v)
+// : GTot Type0
+// = live_region h a.aref_region
+//   /\ Heap.aref_live_at (Map.sel h.h a.aref_region) a.aref_aref v rel
+
+// abstract
+// let greference_of
+//   (a: aref)
+//   (v: Type)
+//   (rel: preorder v)
+// : Ghost (mreference v rel)
+//   (requires (exists h . aref_live_at h a v rel))
+//   (ensures (fun _ -> True))
+// = MkRef a.aref_region (Heap.gref_of a.aref_aref v rel)
+
+// abstract
+// let reference_of
+//   (h: mem)
+//   (a: aref)
+//   (v: Type)
+//   (rel: preorder v)
+// : Pure (mreference v rel)
+//   (requires (aref_live_at h a v rel))
+//   (ensures (fun x -> aref_live_at h a v rel /\ frameOf x == frameOf_aref a /\ as_addr x == aref_as_addr a /\ is_mm x == aref_is_mm a))
+// = MkRef a.aref_region (Heap.ref_of (Map.sel h.h a.aref_region) a.aref_aref v rel)
+
+// abstract
+// let aref_live_at_aref_of
+//   (h: mem)
+//   (#t: Type0)
+//   (#rel: preorder t)
+//   (r: mreference t rel)
+// : Lemma
+//   (aref_live_at h (aref_of r) t rel <==> contains h r)
+//   [SMTPat (aref_live_at h (aref_of r) t rel)]
+// = ()
+
+// abstract
+// let contains_greference_of
+//   (h: mem)
+//   (a: aref)
+//   (t: Type0)
+//   (rel: preorder t)
+// : Lemma
+//   (requires (exists h' . aref_live_at h' a t rel))
+//   (ensures ((exists h' . aref_live_at h' a t rel) /\ (contains h (greference_of a t rel) <==> aref_live_at h a t rel)))
+//   [SMTPatOr [
+//     [SMTPat (contains h (greference_of a t rel))];
+//     [SMTPat (aref_live_at h a t rel)];
+//   ]]
+// = ()
+
+// abstract
+// let aref_of_greference_of
+//   (a: aref)
+//   (v: Type0)
+//   (rel: preorder v)
+// : Lemma
+//   (requires (exists h' . aref_live_at h' a v rel))
+//   (ensures ((exists h' . aref_live_at h' a v rel) /\ aref_of (greference_of a v rel) == a))
+//   [SMTPat (aref_of (greference_of a v rel))]
+// = ()
+
+// (* Operators lowered to rref *)
+
+// abstract let frameOf_greference_of
+//   (a: aref)
+//   (t: Type)
+//   (rel: preorder t)
+// : Lemma
+//   (requires (exists h . aref_live_at h a t rel))
+//   (ensures ((exists h . aref_live_at h a t rel) /\ frameOf (greference_of a t rel) == frameOf_aref a))
+//   [SMTPat (frameOf (greference_of a t rel))]
+// = ()
+
+// abstract
+// let as_addr_greference_of
+//   (a: aref)
+//   (t: Type0)
+//   (rel: preorder t)
+// : Lemma
+//   (requires (exists h . aref_live_at h a t rel))
+//   (ensures ((exists h . aref_live_at h a t rel) /\ as_addr (greference_of a t rel) == aref_as_addr a))
+//   [SMTPat (as_addr (greference_of a t rel))]
+// = ()
+
+// abstract
+// let is_mm_greference_of
+//   (a: aref)
+//   (t: Type0)
+//   (rel: preorder t)
+// : Lemma
+//   (requires (exists h . aref_live_at h a t rel))
+//   (ensures ((exists h . aref_live_at h a t rel) /\ is_mm (greference_of a t rel) == aref_is_mm a))
+//   [SMTPat (is_mm (greference_of a t rel))]
+// = ()
+
+// abstract
+// let unused_in_greference_of
+//   (a: aref)
+//   (t: Type0)
+//   (rel: preorder t)
+//   (h: mem)
+// : Lemma
+//   (requires (exists h . aref_live_at h a t rel))
+//   (ensures ((exists h . aref_live_at h a t rel) /\ (unused_in (greference_of a t rel) h <==> aref_unused_in a h)))
+//   [SMTPat (unused_in (greference_of a t rel) h)]
+// = ()
+
+// abstract
+// let sel_reference_of
+//   (a: aref)
+//   (v: Type0)
+//   (rel: preorder v)
+//   (h1 h2: mem)
+// : Lemma
+//   (requires (aref_live_at h1 a v rel /\ aref_live_at h2 a v rel))
+//   (ensures (aref_live_at h2 a v rel /\ sel h1 (reference_of h2 a v rel) == sel h1 (greference_of a v rel)))
+//   [SMTPat (sel h1 (reference_of h2 a v rel))]
+// = ()
+
+// abstract
+// let upd_reference_of
+//   (a: aref)
+//   (v: Type0)
+//   (rel: preorder v)
+//   (h1 h2: mem)
+//   (x: v)
+// : Lemma
+//   (requires (aref_live_at h1 a v rel /\ aref_live_at h2 a v rel))
+//   (ensures (aref_live_at h1 a v rel /\ aref_live_at h2 a v rel /\ upd h1 (reference_of h2 a v rel) x == upd h1 (greference_of a v rel) x))
+//   [SMTPat (upd h1 (reference_of h2 a v rel) x)]
+// = ()
